theories/FOL/Reductions/PCPb_to_FOL_intu.v
@@ -1,6 +1,6 @@
 (** * Intuitionistic FOL *)
 
-From Undecidability.FOL Require Import Kripke PCPb_to_FOL FOL.
+From Undecidability.FOL Require Import Kripke PCPb_to_FOL.
 
 Require Import Undecidability.PCP.Reductions.PCPb_iff_dPCPb.
 (** ** Reductions *)
@@ -9,17 +9,14 @@ Section kvalidity.
 
   Local Definition BSRS := list (card bool).
   Variable R : BSRS.
-  Context {b : logic}.
-    
-  Set Printing Implicit.
+  Context {ff : falsity_flag}.
 
   Theorem BPCP_kprv :
     PCPb R <-> nil ⊢I (F R).
   Proof.
     rewrite PCPb_iff_dPCPb. split.
     - apply BPCP_prv'.
-    - intros H. About prv.
-    eapply ksoundness' with (A := []) (phi := F R) in H. rewrite <- PCPb_iff_dPCPb. now apply (BPCP_valid R), kvalid_valid.
+    - intros H % ksoundness'. rewrite <- PCPb_iff_dPCPb. now apply (BPCP_valid R), kvalid_valid.
   Qed.
 
   Theorem BPCP_kvalid :
@@ -37,8 +34,8 @@ Theorem BPCP_ksatis R :
 Proof.
   split.
   - intros H % (BPCP_satis R). now apply ksatis_satis.
-  - intros (D & eta & M & u & rho & H) H' % (BPCP_kvalid R (b:=full)).
-    now apply (H u), (H' D eta M u).
+  - intros (D & M & u & rho & H) H' % (BPCP_kvalid R (ff:=falsity_on)).
+    apply (H u), (H' D M u). apply M.
 Qed.
 
 (** Reduction theorems  *)
@@ -64,38 +61,38 @@ Qed.
 (** ** Corollaries *)
 
 Corollary kvalid_undec :
-  UA -> ~ decidable (@kvalid full).
+  UA -> ~ decidable (@kvalid _ _ falsity_on).
 Proof.
   intros H. now apply (not_decidable kvalid_red).
 Qed.
 
 Corollary kvalid_unenum :
-  UA -> ~ enumerable (compl (@kvalid full)).
+  UA -> ~ enumerable (compl (@kvalid _ _ falsity_on)).
 Proof.
   intros H. now apply (not_coenumerable kvalid_red).
 Qed.
 
 Corollary kprv_undec :
-  UA -> ~ decidable (@prv intu full nil).
+  UA -> ~ decidable (@prv _ _ falsity_on intu nil).
 Proof.
   intros H. now apply (not_decidable kprv_red).
 Qed.
 
 Corollary kprv_unenum :
-  UA -> ~ enumerable (compl (@prv intu full nil)).
+  UA -> ~ enumerable (compl (@prv _ _ falsity_on intu nil)).
 Proof.
   intros H. apply (not_coenumerable kprv_red); trivial.
 Qed.
 
 Corollary ksatis_undec :
-  UA -> ~ decidable (@ksatis full).
+  UA -> ~ decidable (@ksatis _ _ falsity_on).
 Proof.
   intros H1 H2 % (dec_red ksatis_red).
   now apply H1, dec_count_enum.
 Qed.
 
 Corollary ksatis_enum :
-  UA -> ~ enumerable (@ksatis full).
+  UA -> ~ enumerable (@ksatis _ _ falsity_on).
 Proof.
   intros H1 H2 % (enumerable_red ksatis_red); auto.
 Qed.
